Added Performance.s.dfy with necessary changes and cleaned up unnecessary files

ironfleet/src/Dafny/Distributed/Protocol/Lock/Types.i.dfy
@@ -6,8 +6,9 @@ import opened Environment_s
 import opened Native__Io_s
 
 datatype LockMessage = Transfer(transfer_epoch:int) | Locked(locked_epoch:int) | Invalid
+datatype LockStep = GrantStep | AcceptStep
 
-type LockEnvironment = LEnvironment<EndPoint, LockMessage>
+type LockEnvironment = LEnvironment<EndPoint, LockMessage, LockStep>
 type LockPacket = LPacket<EndPoint, LockMessage>
 type LockIo = LIoOp<EndPoint, LockMessage>
 
